tests/bug-reports/Bug1287.fst
@@ -99,7 +99,7 @@ let term_head t : string =
   | Tv_App f x -> "Tv_App"
   | Tv_Abs x t -> "Tv_Abs"
   | Tv_Arrow x t -> "Tv_Arrow"
-  | Tv_Type () -> "Tv_Type"
+  | Tv_Type u -> "Tv_Type"
   | Tv_Refine x t -> "Tv_Refine"
   | Tv_Const cst -> "Tv_Const"
   | Tv_Uvar i t -> "Tv_Uvar"
@@ -170,7 +170,7 @@ let rec interp_pattern_aux (pat: pattern) (cur_bindings: bindings) (tm:term)
     | _ -> raise (SimpleMismatch (pat, tm)) in
   let interp_type cur_bindings tm =
     match inspect tm with
-    | Tv_Type () -> return cur_bindings
+    | Tv_Type u -> return cur_bindings
     | _ -> raise (SimpleMismatch (pat, tm)) in
   let interp_app (p_hd p_arg: (p:pattern{p << pat})) cur_bindings tm =
     match inspect tm with
@@ -329,7 +329,7 @@ let rec pattern_of_term_ex tm : match_res pattern =
   | Tv_FVar fv ->
     let qn = inspect_fv fv in
     return (if qn = any_qn then PAny else PQn qn)
-  | Tv_Type () ->
+  | Tv_Type u ->
     return PType
   | Tv_App f (x, _) ->
     let is_any = match inspect f with
