tests/tactics/Syntax.fst
@@ -54,7 +54,7 @@ let rec blah (t : term) : Tac term =
              | Tv_Arrow b t -> Tv_Arrow b t
              | Tv_Refine b t -> let t = blah t in
                                 Tv_Refine b t
-             | Tv_Type u -> Tv_Type ()
+             | Tv_Type u -> Tv_Type u
              | Tv_Const c -> Tv_Const c
              | Tv_Uvar u t -> Tv_Uvar u t
              | Tv_Let r attrs b t1 t2 -> Tv_Let r attrs b t1 t2
